theories/Projection.v
@@ -2,10 +2,11 @@ From mathcomp Require Import all_ssreflect zify.
 From mathcomp Require Import finmap.
 
 
+From Dep Require Export NewSyntax Substitutions.
+
+(*Let inE := NewSyntax.inE.*)
+
 From Equations Require Import Equations.
-
-From Dep Require Import NewSyntax Bisimulation.
-
 
 Lemma esize0 : forall e, 1 <= esize e.
 Proof.
@@ -138,46 +139,9 @@ Set Implicit Arguments.
 Unset Strict Implicit.
 Unset Printing Implicit Defensive.
 
-Check in_left. Print Sumbool.sumbool_of_bool.
-(*Lemma unfeq_elim2
-     : forall P : endpoint -> endpoint -> bool -> Type,
-       (forall n0 n1 : fin, P (EVar n0) (EVar n1) (n0 == n1)) ->
-       (forall n : fin, P (EVar n) EEnd false) ->
-       (forall (n : fin) (d : dir) (c : ch) (v : value) (e : endpoint), P (EVar n) (EMsg d c v e) false) ->
-       (forall (n : fin) (d0 : dir) (c0 : ch) (l : seq endpoint), P (EVar n) (EBranch d0 c0 l) false) ->
-       (forall (n : fin) (e0 : endpoint), P (EVar n) (ERec e0) false) ->
-       (forall e : endpoint, P EEnd e (is_mue e)) ->
-       (forall (d : dir) (c : ch) (v : value) (e : endpoint) (n : fin), P (EMsg d c v e) (EVar n) false) ->
-       (forall (d : dir) (c : ch) (v : value) (e : endpoint), P (EMsg d c v e) EEnd false) ->
-       (forall (d0 : dir) (c0 : ch) (v0 : value) (e0' : endpoint) (d1 : dir) (c1 : ch) (v1 : value) (e1' : endpoint),
-        P e0' e1' (unfeq e0' e1') -> P (EMsg d0 c0 v0 e0') (EMsg d1 c1 v1 e1') ((d0 == d1) && (c0 == c1) && (v0 == v1) && unfeq e0' e1')) ->
-       (forall (d : dir) (c : ch) (v : value) (e : endpoint) (d1 : dir) (c1 : ch) (l : seq endpoint), P (EMsg d c v e) (EBranch d1 c1 l) false) ->
-       (forall (d : dir) (c : ch) (v : value) (e e1 : endpoint), P (EMsg d c v e) (ERec e1) false) ->
-       (forall (d0 : dir) (c0 : ch) (l : seq endpoint) (n : fin), P (EBranch d0 c0 l) (EVar n) false) ->
-       (forall (d0 : dir) (c0 : ch) (l : seq endpoint), P (EBranch d0 c0 l) EEnd false) ->
-       (forall (d0 : dir) (c0 : ch) (l : seq endpoint) (d : dir) (c : ch) (v : value) (e : endpoint), P (EBranch d0 c0 l) (EMsg d c v e) false) ->
-       (forall (d0 : dir) (c0 : ch) (es0 : seq endpoint) (d1 : dir) (c1 : ch) (es1 : seq endpoint),
-        (forall e0 e1 : endpoint, In e0 es0 -> In e1 es1 -> P e0 e1 (unfeq e0 e1)) ->
-        P (EBranch d0 c0 es0) (EBranch d1 c1 es1) ((d0 == d1) && (c0 == c1) && list_eq unfeq es0 es1)) ->
-       (forall (d0 : dir) (c0 : ch) (l : seq endpoint) (e0 : endpoint), P (EBranch d0 c0 l) (ERec e0) false) ->
-       (forall (e0' : endpoint) (e : econtractive2 (ERec e0') = true) (n : fin),
-        P e0' [e(ERec e0')..] (EVar n) (unfeq e0' [e(ERec e0')..] (EVar n)) ->   econtractive2 (ERec e0')  -> P (ERec e0') (EVar n) (unfeq e0' [e(ERec e0')..] (EVar n))) ->
-       (forall (e0' : endpoint) (e : econtractive2 (ERec e0') = true),
-        P e0' [e(ERec e0')..] EEnd (unfeq e0' [e(ERec e0')..] EEnd) ->  econtractive2 (ERec e0') ->  P (ERec e0') EEnd (unfeq e0' [e(ERec e0')..] EEnd)) ->
-       (forall (e0' : endpoint) (e : econtractive2 (ERec e0') = true) (d : dir) (c : ch) (v : value) (e0 : endpoint),
-        P e0' [e(ERec e0')..] (EMsg d c v e0) (unfeq e0' [e(ERec e0')..] (EMsg d c v e0)) ->  econtractive2 (ERec e0') -> P (ERec e0') (EMsg d c v e0) (unfeq e0' [e(ERec e0')..] (EMsg d c v e0))) ->
-       (forall (e0' : endpoint) (e : econtractive2 (ERec e0') = true) (d0 : dir) (c0 : ch) (l : seq endpoint),
-        P e0' [e(ERec e0')..] (EBranch d0 c0 l) (unfeq e0' [e(ERec e0')..] (EBranch d0 c0 l)) ->  econtractive2 (ERec e0') -> P (ERec e0') (EBranch d0 c0 l) (unfeq e0' [e(ERec e0')..] (EBranch d0 c0 l))) ->
-       (forall (e0' : endpoint) (e : econtractive2 (ERec e0') = true) (e1' : endpoint),
-        P e0' e1' (unfeq e0' e1') ->
-        P e0' [e(ERec e0')..] (ERec e1') (unfeq e0' [e(ERec e0')..] (ERec e1')) ->  econtractive2 (ERec e0') ->  P (ERec e0') (ERec e1') (unfeq e0' e1' || unfeq e0' [e(ERec e0')..] (ERec e1'))) ->
-       (forall (e0' : endpoint) (e0 : econtractive2 (ERec e0') = false) (e1 : endpoint), P (ERec e0') e1 false) -> forall e0 e1 : endpoint, P e0 e1 (unfeq e0 e1).
-Proof.
-intros. apply unfeq_elim;eauto.
-intros. split_and. rewrite /= list_eqP. eauto. 
-Qed.*)
 
-Let inE := NewSyntax.inE.
+
+
 
 
 Fixpoint project g p := 
@@ -223,6 +187,17 @@ move=>->. apply H. intro. intros. destruct x1;destruct x2;try done. inversion H2
 done. 
 Qed.
 
+
+(*Lemma injective_lift_ren : forall sigma, injective sigma -> injective (0 .: sigma >> succn). 
+Proof. 
+intros. intro. case. simpl. destruct x1.  done.  simpl.  done.
+intro.  simpl. destruct x1. done. simpl. intros. f_equal. apply H. inversion H0. done. 
+Qed. 
+
+Lemma injective_shift : injective S.
+Proof. intro. intros. inversion H.  done. Qed.
+
+Hint Resolve injective_shift  injective_lift_ren.*)
 
 
 Lemma eguarded_shift2 : forall g i sigma, injective sigma ->  eguarded (sigma i) g ⟨e sigma⟩ ->  eguarded i g.
@@ -309,6 +284,27 @@ done.  move : H. asimpl. done. f_equal. move : H. asimpl. case. move/H1. done. *
 Qed.
 
 
+
+Lemma inj_rem : forall e0 e1 f f', injective f  -> e0 ⟨e f⟩ = e1 ⟨e f⟩ -> e0 ⟨e f' ⟩ = e1 ⟨e f' ⟩.
+Proof. 
+elim. intros. destruct e1;try done.  f_equal. move : H0. asimpl. case. move/H. by move=>->. 
+- case;try done.
+- intros. asimpl.  destruct e1;try done. f_equal. move : H1.  asimpl. intros. f_equal. 
+  apply : H. have : injective (0 .: f >> succn ).
+  intro. intros. destruct x1;destruct x2. done. move : H.  asimpl.
+done.  move : H. asimpl. done. f_equal. move : H. asimpl. case. move/H0. done. move => HH. apply : HH. 
+
+(*intro. intros. destruct x1;destruct x2. done. move : H.  asimpl.
+done.  move : H. asimpl. done. f_equal. move : H. asimpl. case. move/H1. done. *)
+  move : H1.  asimpl. case. intros. eauto.
+- intros. destruct e1;try done.
+ move : H1.  asimpl. case. intros.  subst. f_equal. eauto. 
+- intros. move : H1.  asimpl. destruct e1;try done. asimpl. case. intros. subst. f_equal.
+  move : H3. elim : l l0 H;simpl. destruct l0. done. done. destruct l0. done. 
+  simpl. intros. f_equal. apply : H1. auto. eauto. inversion H3. done.  apply H. 
+  intros. apply : H1. eauto. eauto. eauto.  inversion H3. eauto. 
+Qed.
+
 Lemma inj_rem2 : forall e0 e1 f , injective f  -> e0 ⟨e f⟩ = e1 ⟨e f⟩ -> e0 = e1.
 Proof. intros. have : e0 = e0 ⟨id⟩.  asimpl. done. move=>->. 
 have : e1 = e1 ⟨id⟩. asimpl. done. move=>->. apply/inj_rem. eauto. eauto.
@@ -338,13 +334,10 @@ elim;intros.
 - done.
 - simpl. asimpl. rewrite H. symmetry. case_if.
   * asimpl. case_if. done. have : 0 = (0.: sigma >> succn ) 0. done. intros. rewrite {1}x in H2.
-    eapply eguarded_shift in H1. erewrite H1 in H2. done. apply inject2.  done. 
+    eapply eguarded_shift in H1. erewrite H1 in H2. done. auto. 
     case_if. have : 0 = (0.: sigma >> succn ) 0. done. intros. rewrite {1}x in H2. 
-    apply eguarded_shift in H2. rewrite H2 in H1. done. apply inject2. done. simpl in *. done.
-(*    f_equal.  asimpl. apply inj_rem4'. intros. apply eguarded_fv2 in H1.  rewrite /= H1 in H3. 
-    rewrite /= inE in H3.  rewrite /= (eqP H3). simpl in *. done.*)
-
-    apply inject2.  done.
+    apply eguarded_shift in H2. rewrite H2 in H1. done. auto. done. simpl in *. auto. 
+    auto. 
 - simpl in *.
 rifliad;asimpl;try done. f_equal. auto.  f_equal. auto. auto.
 simpl. rifliad;asimpl;try done. f_equal. rewrite -!map_comp. apply/eq_in_map=>l'. intros. simpl.
@@ -399,7 +392,7 @@ intros. intro. move : x1 sigma H. elim; intros.
 destruct x2; simpl in *. inversion H0. f_equal. apply H. done. all : try done.
 destruct x2; simpl in *. inversion H0. done. all : try done.
 destruct x2; simpl in *. all : try done. f_equal. inversion H1. apply : H. 2 : {  eauto.  }
-asimpl. apply inject2.  done. simpl in *. destruct x2; try done. simpl in *. inversion H1. subst. f_equal.  
+asimpl. auto. simpl in *. destruct x2; try done. simpl in *. inversion H1. subst. f_equal.  
 apply : H. eauto. done.  
 destruct x2; try done. simpl in *. inversion H1. subst. f_equal.  
 move : H4. clear H1. move : l l0 H. elim. intros. destruct l0. done. simpl in *.  done.
@@ -482,49 +475,6 @@ Definition fresh (S : fset_ptcp) :=
     end.
 
 
-(*
-Fixpoint unfeq sigma e0 e1:= 
-  match e0,e1 with 
-  | EVar n0, EVar n1 => n0 == n1 
-  | EEnd, EEnd => true
-  | EMsg d0 c0 v0 e0', EMsg d1 c1 v1 e1' => (d0 == d1) && (c0 == c1) && (v0 == v1) && (unfeq sigma e0' e1')
-  | EBranch d0 c0 es0, EBranch d1 c1 es1 => (d0 == d1) && (c0 == c1) && (list_eq (unfeq sigma) es0 es1)
-  | ERec e0', _ => (if e1 is ERec e1' then unfeq ((var 0) : sigma) e0' e1' else false) || (unfeq n' (e0' [e (ERec e0').:ids]) e1)
-  | _,_ => false  
-end
-else false.*)
-
-
-Print endpoint. 
-
-
-Require Import Coq.Program.Wf Program.
-Print lt. 
-(*Use equations because it supports nested well founded recursion*)
-
-
-
-
-(*
-(*from https://mattam82.github.io/Coq-Equations/examples/Examples.STLC.html
- just the definition of lexicografic*)
-
-Require Import Arith Wf_nat.
-Instance wf_nat : Classes.WellFounded lt := lt_wf.
-Hint Constructors Subterm.lexprod : subterm_relation.
-
-Derive Signature for Acc.
-Notation lexicographic R S := (Subterm.lexprod _ _ R S).
-*)
-
-
-(*Fixpoint unfeq2 e0 e1 :=
-match e0,e1 with
-| EBranch d c es, EBranch d' c' es' => (d == d') || (c == c') || (list_eq unfeq2 es es')
-
- unfeq e0 e1 || unfeq e1 e0.
-
-Definition unfeq2 e0 e1 := unfeq e0 e1 || unfeq e1 e0.*)
 
 
 Fixpoint project_pred  (g : gType):=  
@@ -539,241 +489,3 @@ match g with
 | GRec g0 => project_pred g0
 | _ => true 
 end.
-
-
-
-
-
-(*Lemma endpoint_rename : forall e,  endpoint_fv (ren_endpoint predn e) = predn @` endpoint_fv e.
-Proof. 
-elim;rewrite /=;intros. rewrite Imfset.imfsetE /=. fsetTac. rewrite seq_fsetE.
-apply bool_iff. split. move/eqP=>->. rewrite map_f //=. rewrite !inE //=. 
-move/mapP=>[]. intros. rewrite !inE in p. rewrite -(eqP p) -q //= eqxx //=.
-simpl inrewrite predn_fset0 //=.
-f_equal.*)
-
-(*Lemma fv_shiftdown : forall e i, i \notin (endpoint_fv i e)  -> endpoint_fv i (shiftdown e) = endpoint_fv i.+1 e.
-Proof. 
-elim;rewrite /=;try done;intros.
-move : H. rifliad;rewrite !inE;intros. all : try fsetTac. 
-rewrite -H //=. asimpl.  rewrite /shiftdown.
- asimpl. f_equal. clear H0. clear H. rewrite /scons.
-fext.  intros. 
-Admitted.
-*)
-
-(*Lemma fv_predn : forall e, endpoint_fv e ⟨ predn ⟩ = [fset predn n | n in endpoint_fv e].
-Proof. intros. fsetTac. destruct (k \in endpoint_fv e ⟨ predn ⟩) eqn:Heqn;rewrite Heqn /= bbrw.
-apply/imfsetP.
-elim : e k Heqn;intros.
-- exists n. rewrite /= !inE //=. move : Heqn. rewrite /= !inE //=. lia.
-- rewrite /= !inE //= in Heqn. 
-- rewrite /= ?inE in Heqn.
-  exists k. rewrite /=. move : Heqn. asimpl. move => HH.  
-  have :  (k \in endpoint_fv e ⟨e predn ⟩). admit. move/H=>[]. move => x. simpl.
-  intros. apply/imfsetP. exists x. simpl. rewrite !inE /=. split_and. 
-  have : ( 0 .: predn >> succn ) = (0 .: id). fext. intros.  case. done. intros. simpl. destruct n. asimpl.  simpl. done.
-asimpl_in Heqn. rewrite /= !inE //=. move : Heqn. rewrite /= !inE //=. lia.
-
- -
-  elim;intros.
-fsetTac. destruct (eqVneq k n.-1). rewrite bbrw.  
-apply/imfsetP. exists n. simpl. rewrite !inE //=. done. 
-rewrite bbrw.  move/imfsetP. move=>[] x. simpl. rewrite !inE. move/eqP=>->. lia. 
-simpl. fsetTac. rewrite bbrw. move/imfsetP=>[] x. simpl. rewrite !inE //=.
-fsetTac. asimpl.*)
-
-(*Lemma subst_nop : forall e e' x, x \notin (fv e) -> subst_e x e e' = e. Proof. 
-elim;rewrite /=;try done;intros. move : H. rewrite !inE.  rewrite neg_sym. move/negbTE=>->. done. 
-move : H0. rewrite !inE. move/orP=>[]. by rewrite eq_sym=>->.  
-intros. rifliad. rewrite H //=. 
-f_equal. auto. f_equal. rewrite big_map in H0.  induction l. done. simpl. f_equal.  apply H.  rewrite !inE.  lia. simpl in H0. move : H0. 
-rewrite big_cons. rewrite !inE. split_and. apply IHl. intros. apply H. rewrite !inE H1. lia. done. move : H0.  rewrite big_cons !inE. split_and. 
-Qed.*)
-
-
-
-
-(*Lemma fv_subst : forall  e e' n x, fv e' = fset0 -> n <> x -> (n \in (fv (subst_e x e e'))) = (n \in (fv e)).
-Proof. elim;rewrite /=;try done;intros. rewrite !inE. rifliad. rewrite H !inE. have : n0 == n = false by lia. by move=>->. 
-rewrite /= !inE. done. 
-rifliad. rewrite /=. Check mem_map. Search (_ \in (map _ _)). Search _ (_ \in _ = _ \in _).  Search _ ((is_true _ -> is_true _) -> _ = _). rewrite !inE.  destruct (n0 != n)eqn:Heqn;rewrite /= //=.   rewrite Heqn //=.
-apply H. done. done. rewrite Heqn //=. 
-rewrite !big_map.  elim : l H. rewrite !big_nil. done. intros. rewrite !big_cons. rewrite !inE. rewrite H2 //=. 
-destruct ( (n \in fv a)) eqn:Heqn; rewrite !Heqn //=. apply H. intros. apply H2. rewrite !inE H3. lia. done. done. 
-Qed.*)
-
-(*Lemma fv_nil_evar : forall e n, endpoint_fv 0 e = fset0 -> e <> EVar n. 
-Proof.
-elim;rewrite /=;try  done. intros. have : n \in [fset n]. by  rewrite !inE. move : H. have : n - 0 = n by lia. move=>->. move/fsetP=>->. done. 
-Qed.
-
-Lemma fset_nil : forall (A : choiceType) (n : A), [fset n] = fset0 -> False.
-Proof. intros. move : H. move/fsetP=>HH. suff : n \in [fset n] = (n \in fset0). rewrite !inE eqxx //=. done. 
-Qed.
-*)
-(*Lemma clean_up : forall e sigma, clean (endpoint_ren e S) [↑__endpoint sigma] = (clean e) [↑__endpoint sigma].*)
-
-(*Lemma in_subst : forall e sigma, (endpoint_fv (e [e sigma])) = sigma @` (endpoint_fv e).*)
-
-
-(*Lemma in_subst : forall v e n sigma, v \in (endpoint_fv e) ->  sigma v = EVar n ->  n \in (endpoint_fv (e [e sigma])). 
-Proof. 
-move => v e. elim : e v;asimpl;intros. rewrite !inE in H. rewrite -(eqP H) H0 //= !inE //=. 
-rewrite !inE //= in H.
-rewrite /endpoint_fv -/endpoint_fv. rewrite seq_fsetE. Search _ (_ \in pmap _ _). rewrite mem_pmap. apply/mapP.  exists v. 
-move : H0. rewrite /endpoint_fv -/endpoint_fv.  rewrite seq_fsetE mem_pmap. move/mapP=>[]. intros. apply : H. eauto. 
-destruct x. done.  simpl. asimpl. simpl in q. done. simpl. substify. asimpl.
-
-move : H0. simpl. rewrite mem_map.
-simpl. rewrite fsetE.*)
-
-(*
-
-asimpl. simpl. symmetry. case_if. rewrite -(eqP H2). 
-  move : H1. destruct (clean e);rewrite /=;asimpl. destruct n.  done. simpl. asimpl. destruct (sigma n);rewrite /=;asimpl. 
-  destruct n0. all : try done. rifliad. substify. move/eqP. rewrite /shiftdown. asimpl. move : H1. substify. asimpl. rewrite H. 
-  
-
-have :  subst_endpoint (scons (var 0) (sigma >> (⟨ ↑ ⟩ >> clean)))  == var 0 = false.
-
-case_if. 
-  simpl. case_if. move : H2. 
-asimpl. rs. done.
-- rs. case_if.  
- * rs. rewrite (eqP H1) /=. rifliad. rs. by rewrite /= eqxx. rewrite subst_nop //=. rewrite fv_clean. lia. 
- * rs. rewrite /= H //=.  rewrite fv_subst //=. symmetry. case_if.
-  ** rs. rewrite (eqP H2) /=. rs. rewrite H1 eqxx. done.
-  ** case_if.
-   *** rs. rewrite /= H1. rifliad. exfalso. move : H4.  destruct (clean e);rewrite /=;rs. rifliad. move/eqP. apply : fv_nil_evar. 
-       rewrite fv_clean //=. by rewrite H2. done. done. done. rifliad. 
-
-   *** rs. rifliad. exfalso. move : H5. rewrite !inE H3. have : n != x by lia. move=>->. done. rewrite !inE H3.
-       have : n != x by lia. move=>-> /=. rifliad. 
-       destruct (clean e);rewrite /=;rs.  rifliad. rewrite (eqP H5) in H4. rs_in H4. rewrite eqxx in H4. rewrite -fv_clean in H0.  rewrite (eqP H4) in H0. rs_in H0. by apply fset_nil in H0. rs_in H4. rewrite H5 in H4. lia. done.
-      all : try  by move : (eqP H4).   rs_in H4. rifliad. rs. f_equal. auto.  rs. f_equal. 
-- rewrite -!map_comp. apply/eq_in_map. move => ll Hin /=. rewrite H //=.
-Qed.
-
-Lemma clean_subst : forall (e0 : endpoint)  e' x, endpoint_fv 0 e' = fset0 -> clean (e0[s e'//x]) = (clean e0)[s clean e'//x].
-Proof.
-elim;intros. 
-- rs. rifliad.
-- rs. done.
-- rs. case_if.  
- * rs. rewrite (eqP H1) /=. rifliad. rs. by rewrite /= eqxx. rewrite subst_nop //=. rewrite fv_clean. lia. 
- * rs. rewrite /= H //=.  rewrite fv_subst //=. symmetry. case_if.
-  ** rs. rewrite (eqP H2) /=. rs. rewrite H1 eqxx. done.
-  ** case_if.
-   *** rs. rewrite /= H1. rifliad. exfalso. move : H4.  destruct (clean e);rewrite /=;rs. rifliad. move/eqP. apply : fv_nil_evar. 
-       rewrite fv_clean //=. by rewrite H2. done. done. done. rifliad. 
-
-   *** rs. rifliad. exfalso. move : H5. rewrite !inE H3. have : n != x by lia. move=>->. done. rewrite !inE H3.
-       have : n != x by lia. move=>-> /=. rifliad. 
-       destruct (clean e);rewrite /=;rs.  rifliad. rewrite (eqP H5) in H4. rs_in H4. rewrite eqxx in H4. rewrite -fv_clean in H0.  rewrite (eqP H4) in H0. rs_in H0. by apply fset_nil in H0. rs_in H4. rewrite H5 in H4. lia. done.
-      all : try  by move : (eqP H4).   rs_in H4. rifliad. rs. f_equal. auto.  rs. f_equal. 
-- rewrite -!map_comp. apply/eq_in_map. move => ll Hin /=. rewrite H //=.
-Qed.*)
-
-(*Lemma rproject_subst : forall g g0 p i,  rproject (g[s g0//i]) p = (rproject g p)[s (rproject g0 p)//i].
-Proof. elim;rewrite /=;try done;intros;rs. rifliad. rifliad. rewrite /=.  rewrite H. done.  
-rifliad. simpl. rs. f_equal. done. simpl. rs. f_equal. done. 
-rifliad. simpl. rs. f_equal. 
-rewrite -!map_comp. apply/eq_in_map. move=>ll Hin. simpl. apply H.  done. 
-simpl. rs.  f_equal.
-rewrite -!map_comp. apply/eq_in_map. move=>ll Hin. simpl. apply H.  done. destruct l. done. simpl. apply H. rewrite !inE. done. 
-Qed.*)
-
-(*
-Lemma fv_rename : forall e f, endpoint_fv e ⟨ f ⟩ = [fset f n | n in (endpoint_fv e)].
-Proof.
-elim;rewrite /=;intros. fsetTac. destruct (eqVneq k (f n));rewrite bbrw.
-apply/imfsetP. exists n. rewrite /= !inE eqxx. done. done.
-move/imfsetP=>[] x.  rewrite /= !inE. move/eqP=>->. lia.
-rewrite predn_fset0 //=. asimpl. Print up_ren. 
-fsetTac. symmetry. destruct ( (k \in f @` [fset n.-1 | n in endpoint_fv e & n != 0])) eqn:Heqn;rewrite Heqn bbrw.
-move : Heqn. move/imfsetP=>[] x /= H' H2. subst.  move : H'. move/imfsetP=>[] x0 /=. rewrite !inE /=.
-split_and. subst.  rewrite H. 
-simpl. apply/imfsetP. exists x0. rewrite /= !inE H1  andbC /=. rewrite H. 
-apply/imfsetP. exists x0. simpl. done. destruct x0.  done. simpl. have : f = predn. admit. move=>->. destruct x0. done. asimpl. simpl. move : H'.rewrite !inE. split_and.  exists x0.  done. rewrite H2 q. destruct x0. done. 
- simpl.  asimpl. admit.
-done. simpl. asimpl. 
-simpl in q. subst.  simpl.
-Lemma fv_clean : forall e, endpoint_fv (clean e) = endpoint_fv e. 
-Proof. elim;try solve [rewrite /=;try done];intros. 
-rewrite /=. rifliad;simpl. 
-fsetTac. rewrite (eqP H0) /= in H. rewrite -H.   rewrite bbrw. move/imfsetP=>[] x. simpl. rewrite !inE. split_and. lia.
-rewrite H. done. fsetTac. 
-rewrite H. fsetTac.
-
-rewrite (eqP H0) in H. simpl. simpl in H. rewrite -H. simpl in H.
-fsetTac. apply/negP/negP. move=>_. move/imfsetP=>[]. move => x. simpl. rewrite !inE. split_and. lia. done. 
-rewrite /shiftdown.  *)
-
-
-
-
-
-
-
-
-
-
-
-
-(*Fixpoint same_vars (e : endpoint ) :=
-match e with 
-| EBranch d c l => all (fun e' => endpoint_fv (nth EEnd l 0) == endpoint_fv e') l && (all same_vars l)
-| EMsg _ _ _ e0 => same_vars e0
-| ERec e0 => same_vars e0
-| _ => true 
-end.
-
-Fixpoint same_varsg (e : gType ) :=
-match e with 
-| GBranch c l => all (fun e' => gType_fv (nth GEnd l 0) == gType_fv e') l && (all same_varsg l)
-| GMsg _ _ e0 => same_varsg e0
-| GRec e0 => same_varsg e0
-| _ => true 
-end.*)
-
-
-
-
-(*Lemma in_foldr : forall l n,  n \in foldr (fun g' : gType => cat (fv_g g')) nil l ->  exists g, g \in l /\ n \in (fv_g g).
-Proof. elim;try done;move => l n H n'.
-rewrite /= mem_cat. move/orP=>[]. intros. exists l. rewrite !inE /= a. auto.
-move/H. move=>[] x [].  intros. exists x. rewrite !inE a b. lia. Qed.*)
-
-(*Lemma in_foldr2 : forall l n p g, g \in l -> n \in (fv (project  g p)) ->  n \in foldr (fun g' : gType => cat (fv (project g' p))) nil l.
-Proof. elim;try done;intros. move : H0.
-rewrite !inE. move/orP=>[]. move/eqP. intros. subst. simpl. rewrite mem_cat H1. done. intros.  simpl. rewrite mem_cat. apply/orP. right. apply : H. eauto. done. 
-Qed.*)
-
-
-(*
-Lemma fv_project_in : forall g p n, lpreds rec_pred g ->  (n \in (fv_g g)) -> (n  \in (fv (project g p))).
-Proof.
-elim;rewrite //=;intros. move : H1. rewrite !inE.  split_and. apply (H p) in H3;last cc.
-- rifliad. rewrite (eqP H1) in H3. simpl in H3. rewrite !inE in H3. lia. 
-  simpl. Admitted. 
-(*rewrite !inE.  split_and. 
-- apply (H p) in H1;last cc. rifliad.
-- rifliad. simpl. rewrite !big_map. 
-  apply : big_cup_in.  intros. apply : H. done. cc. cc. apply/big_cup_in.  intros. apply : H4.  apply/big_cup_in. intros. apply : H4. rewrite big_map in H1. done. 
-  rewrite /= !big_map.  apply : big_cup_in.  intros. apply : H. done. cc. eauto. rewrite big_map in H1. done. 
-- rewrite match_n. apply H. cc. cc. move : H1. rewrite big_map foldr_exists. move/hasP=>[] x. intros. 
-  intros.  move : p0. move/nthP=>Hnth. specialize Hnth with GEnd. destruct Hnth.
-
-  apply : fv_rproject_in. 
-  erewrite project_predP. apply : H. apply/mem_nth. apply : H1. cc. rewrite H4.  done. eauto.  cc.   all:cc. instantiate (1 := fresh a). rewrite /fresh. destruct (atom_fresh_for_list a). apply/negP.  move => HH. apply n0. destruct a. move : HH. rewrite !inE.  done. 
-Qed.*)
-
-Lemma fv_project_eq : forall g p n, lpreds rec_pred g ->  (n \in fv_g g) = (n \in fv (project g p)).
-Proof. intros. destruct ( (n \in fv_g g)) eqn:Heqn. rewrite fv_project_in //=.
-destruct ((n \in fv (project g p))) eqn:Heqn2. erewrite fv_rproject_in in Heqn. done. eauto. done. 
-Qed.*)
-
-
-
-
